teaching/taltech2019/ex/hw/FileSystemClient.fst
@@ -1,0 +1,49 @@
+module FileSystemClient
+
+open FileSystem
+
+open FStar.List.Tot
+
+[@expect_failure]
+let test1 (p:path) : FS unit
+                        (requires (fun fs0 -> fs0 == None []))
+                        (ensures  (fun fs0 _ fs1 -> fs0 == fs1)) =
+  create_dir p;
+  show
+  delete p
+
+[@expect_failure]
+let test2 (p:path) : FS (list path)
+                        (requires (fun fs0 -> fs0 == None []))
+                        (ensures  (fun fs0 ps fs1 -> 
+                                     fs0 == fs1 /\
+                                     count p ps == 1)) =
+  create_dir p;
+  let ps = show () in
+  delete p;
+  ps
+
+[@expect_failure]
+let test3 (p:path) : FS unit 
+                        (requires (fun fs0 -> fs0 == None []))
+                        (ensures  (fun fs0 _ fs1 -> fs0 == fs1)) =
+  create_dir p;
+  delete p
+
+[@expect_failure]
+let test4 (p1 p2 p3:path) : FS unit 
+                               (requires (fun fs0 -> fs0 == None []))
+                               (ensures  (fun fs0 _ fs1 -> fs0 == fs1)) =
+  create_dir p1;
+  create_dir p2;
+  delete p1;
+  create_dir p3;
+  delete p2;
+  delete p3
+
+[@expect_failure]
+let test5 (p1 p2:path) : FS unit
+                        (requires (fun fs0 -> True))
+                        (ensures  (fun _ _ fs1 -> count p1 (show_fs fs1) == 1)) =
+  create_dir p1;
+  create_dir p2
